More fun with typing simple type theory.  Randy P. suggested another proof: that a version of the typing relation with an infinitary hypothesis is equivalent to the original.

examples/lambda/sttScript.sml
@@ -1,13 +1,15 @@
-(* a reasoning problem suggested by Randy Pollack:
-     showing a weakening result for a typing relation over lambda calculus
-     terms.  The typing is that of simple type theory.
+(* reasoning problems suggested by Randy Pollack:
+     1. showing a weakening result for a typing relation over lambda calculus
+        terms.  The typing is that of simple type theory.
+     2. showing that another relation, one with a universally quantified
+        hypothesis, is equivalent to the original.
 *)
 
 open HolKernel boolLib Parse bossLib
 
 open ncLib metisLib BasicProvers
 
-open swapTheory
+open swapTheory ncTheory
 
 val _ = new_theory "stt";
 
@@ -23,8 +25,7 @@ val _ = overload_on("-->", ``funspace``)
    are all disjoint.  Here's the primitive recursive defn. *)
 val valid_ctxt_def = Define`
   (valid_ctxt [] = T) /\
-  (valid_ctxt (xA :: G) = (!A'. ~MEM (FST xA, A') G) /\
-                          valid_ctxt G)
+  (valid_ctxt ((x,A) :: G) = (!A'. ~MEM (x, A') G) /\ valid_ctxt G)
 `;
 val _ = export_rewrites ["valid_ctxt_def"]
 
@@ -59,7 +60,7 @@ val _ = export_rewrites ["MEM_ctxtswap"]
 (* valid_ctxt also respects permutation *)
 val valid_ctxt_swap0 = prove(
   ``!G. valid_ctxt G ==> !x y. valid_ctxt (ctxtswap x y G)``,
-  Induct THEN SRW_TAC [][]);
+  Induct THEN ASM_SIMP_TAC (srw_ss()) [pairTheory.FORALL_PROD]);
 val valid_ctxt_swap = store_thm(
   "valid_ctxt_swap",
   ``valid_ctxt (ctxtswap x y G) = valid_ctxt G``,
@@ -88,6 +89,18 @@ val ctxtFV_MEM = store_thm(
   Induct_on `G` THEN
   ASM_SIMP_TAC (srw_ss() ++ boolSimps.DNF_ss) [pairTheory.FORALL_PROD]);
 
+val ctxtFV_ctxtswap = store_thm(
+  "ctxtFV_ctxtswap",
+  ``ctxtFV (ctxtswap x y G) = swapset x y (ctxtFV G)``,
+  SRW_TAC [][ctxtFV_MEM, pred_setTheory.EXTENSION] THEN
+  METIS_TAC [MEM_ctxtswap, swapstr_def]);
+val _ = export_rewrites ["ctxtFV_ctxtswap"]
+
+val ctxtswap_fresh = store_thm(
+  "ctxtswap_fresh",
+  ``~(x IN ctxtFV G) /\ ~(y IN ctxtFV G) ==> (ctxtswap x y G = G)``,
+  Induct_on `G` THEN ASM_SIMP_TAC (srw_ss()) [pairTheory.FORALL_PROD]);
+
 (* set up parsing/pretty-printing for the typing relation.
    Can't use ":" to the right of the turnstile, because it's already taken
    for HOL's typing, so use "-:" instead, which is ugly. *)
@@ -106,7 +119,7 @@ val (hastype_rules, hastype_ind, hastype_cases) = Hol_reln`
                Gamma |- VAR s -: A) /\
   (!Gamma m n A B. Gamma |- m -: A --> B /\ Gamma |- n -: A ==>
                    Gamma |- m @@ n -: B) /\
-  (!Gamma x m A B. (!A'. ~MEM (x,A') Gamma) /\ (x,A) :: Gamma |- m -: B ==>
+  (!Gamma x m A B. (x,A) :: Gamma |- m -: B ==>
                    Gamma |- LAM x m -: A --> B)
 `;
 
@@ -133,11 +146,19 @@ val subctxt_ctxtFV = store_thm(
   SIMP_TAC (srw_ss()) [pred_setTheory.SUBSET_DEF, subctxt_def] THEN
   METIS_TAC [ctxtFV_MEM]);
 
+val hastype_valid_ctxt = store_thm(
+  "hastype_valid_ctxt",
+  ``!G m A. G |- m -: A ==> valid_ctxt G``,
+  HO_MATCH_MP_TAC hastype_ind THEN SRW_TAC [][]);
+
+val strong_hastype_ind =
+    IndDefRules.derive_strong_induction (CONJUNCTS hastype_rules,
+                                         hastype_ind)
 
 val weakening = store_thm(
   "weakening",
   ``!G m A. G |- m -: A ==> !D. valid_ctxt D /\ G <= D ==> D |- m -: A``,
-  HO_MATCH_MP_TAC hastype_ind THEN REPEAT CONJ_TAC THENL [
+  HO_MATCH_MP_TAC strong_hastype_ind THEN REPEAT CONJ_TAC THENL [
     (* var case *) METIS_TAC [hastype_rules, subctxt_def],
     (* app case *) METIS_TAC [hastype_rules],
 
@@ -145,7 +166,7 @@ val weakening = store_thm(
     (* restatement of goal (with IH etc)  *)
     Q_TAC SUFF_TAC
           `!G v m A B.
-              (!A. ~MEM (v,A) G) /\
+              (v,A) :: G |- m -: B /\
               (!D. valid_ctxt D /\ ((v,A)::G) <= D ==> D |- m -: B) ==>
               !D. valid_ctxt D /\ G <= D ==> D |- LAM v m -: A --> B`
           THEN1 METIS_TAC [] THEN REPEAT STRIP_TAC THEN
@@ -154,9 +175,8 @@ val weakening = store_thm(
     `LAM v m = LAM z (swap z v m)`
        by SRW_TAC [][swap_ALPHA] THEN
     Q_TAC SUFF_TAC
-          `(z,A)::D |- swap z v m -: B /\ (!A. ~MEM (z,A) D)`
+          `(z,A)::D |- swap z v m -: B`
           THEN1 METIS_TAC [hastype_rules] THEN
-    `!A. ~MEM (z,A) D` by METIS_TAC [ctxtFV_MEM] THEN
     `(z,A)::D = ctxtswap z v ((v,A)::ctxtswap z v D)` by SRW_TAC [][] THEN
     Q_TAC SUFF_TAC
           `(v,A)::ctxtswap z v D |- m -: B`
@@ -169,15 +189,118 @@ val weakening = store_thm(
           by (SRW_TAC [][] THEN
               METIS_TAC [MEM_ctxtswap, ctxtFV_MEM, swapstr_def]) THEN
     Q_TAC SUFF_TAC
-          `G <= ctxtswap z v D`
+          `!y B'. MEM (y,B') G ==> MEM (y,B') (ctxtswap z v D)`
           THEN1 (SRW_TAC [][subctxt_def] THEN METIS_TAC []) THEN
+    REPEAT STRIP_TAC THEN
     Q_TAC SUFF_TAC
-          `!y B. MEM (y,B) G ==> MEM (y,B) (ctxtswap z v D)`
-          THEN1 SRW_TAC [][subctxt_def] THEN REPEAT STRIP_TAC THEN
-    Q_TAC SUFF_TAC
-          `~(y = z)`
+          `~(y = z) /\ ~(y = v)`
           THEN1 METIS_TAC [swapstr_def, MEM_ctxtswap, subctxt_def] THEN
+    `~(v IN ctxtFV G)` by METIS_TAC [hastype_valid_ctxt, valid_ctxt_def,
+                                     ctxtFV_MEM] THEN
     METIS_TAC [subctxt_def, ctxtFV_MEM]
   ]);
+
+
+(* now a slightly different typing relation, with different syntax: "||-"
+   instead of "|-".  Underlying name of constant is "hastype2".  *)
+val _ = add_rule {block_style = (AroundEachPhrase, (PP.INCONSISTENT, 2)),
+                  fixity = Infix(NONASSOC, 425),
+                  paren_style = OnlyIfNecessary,
+                  pp_elements = [HardSpace 1, TOK "||-", BreakSpace(1, 0),
+                                 BeginFinalBlock(PP.INCONSISTENT, 2),
+                                 TM, HardSpace 1, TOK "-:", BreakSpace(1,0)],
+                  term_name = "hastype2"}
+
+val (hastype2_rules, hastype2_ind, hastype2_cases) = Hol_reln`
+  (!Gamma s A. valid_ctxt Gamma /\ MEM (s,A) Gamma ==>
+               Gamma ||- VAR s -: A) /\
+  (!Gamma m n A B. Gamma ||- m -: A --> B /\ Gamma ||- n -: A ==>
+                   Gamma ||- m @@ n -: B) /\
+  (!Gamma m x A B. (!v. ~(v IN ctxtFV Gamma) ==>
+                        (v,A) :: Gamma ||- [VAR v/x]m -: B) ==>
+                   Gamma ||- LAM x m -: A --> B)
+`;
+
+val hastype2_swap = store_thm(
+  "hastype2_swap",
+  ``!G m A. G ||- m -: A ==> !x y. ctxtswap x y G ||- swap x y m -: A``,
+  HO_MATCH_MP_TAC hastype2_ind THEN SRW_TAC [][swap_thm] THENL [
+    METIS_TAC [hastype2_rules, MEM_ctxtswap, valid_ctxt_swap],
+    METIS_TAC [hastype2_rules],
+    MATCH_MP_TAC (last (CONJUNCTS hastype2_rules)) THEN
+    SRW_TAC [][swap_subst_out, swap_thm] THEN
+    METIS_TAC [swapstr_def]
+  ]);
+
+val hastype2_valid_ctxt = store_thm(
+  "hastype2_valid_ctxt",
+  ``!G m A. G ||- m -: A ==> valid_ctxt G``,
+  HO_MATCH_MP_TAC hastype2_ind THEN SRW_TAC [][] THEN
+  Q_TAC (NEW_TAC "z") `ctxtFV G` THEN METIS_TAC []);
+
+val hastype_FV = store_thm(
+  "hastype_FV",
+  ``!G m A. G |- m -: A ==> !v. v IN FV m ==> v IN ctxtFV G``,
+  HO_MATCH_MP_TAC hastype_ind THEN SRW_TAC [][] THEN
+  METIS_TAC [ctxtFV_MEM]);
+
+val hastype_swap_eqn = store_thm(
+  "hastype_swap_eqn",
+  ``G |- swap x y m -: A = ctxtswap x y G |- m -: A``,
+  METIS_TAC [hastype_swap, swap_inverse, ctxtswap_involution]);
+
+val hastype2_swap_eqn = store_thm(
+  "hastype2_swap_eqn",
+  ``G ||- swap x y m -: A = ctxtswap x y G ||- m -: A``,
+  METIS_TAC [ctxtswap_involution, hastype2_swap, swap_inverse]);
+
+val hastype2_hastype = prove(
+  ``!G m A. G ||- m -: A ==> G |- m -: A``,
+  HO_MATCH_MP_TAC hastype2_ind THEN REPEAT CONJ_TAC THENL [
+    (* var case *) SRW_TAC [][hastype_rules],
+    (* app case *) METIS_TAC [hastype_rules],
+    (* abs case; first state the goal, with IH etc *)
+    Q_TAC SUFF_TAC
+          `!G m x A B.
+              (!v. ~(v IN ctxtFV G) ==> (v,A) :: G |- [VAR v/x] m -: B) ==>
+              G |- LAM x m -: A --> B` THEN1 METIS_TAC [] THEN
+    REPEAT STRIP_TAC THEN
+    (* fresh z *)
+    Q_TAC (NEW_TAC "z") `FV m UNION ctxtFV G UNION {x}` THEN
+    `LAM x m = LAM z ([VAR z/x] m)`
+       by SRW_TAC [][SIMPLE_ALPHA] THEN
+    METIS_TAC [hastype_rules]
+  ]);
+
+val hastype_hastype2 = prove(
+  ``!G m A. G |- m -: A ==> G ||- m -: A``,
+  HO_MATCH_MP_TAC hastype_ind THEN REPEAT CONJ_TAC THENL [
+    (* var case *) SRW_TAC [][hastype2_rules],
+    (* app case *) METIS_TAC [hastype2_rules],
+    (* abs case; goal with IH is: *)
+    Q_TAC SUFF_TAC
+          `!G x m A B. (x,A) :: G ||- m -: B ==> G ||- LAM x m -: A --> B`
+          THEN1 METIS_TAC [] THEN REPEAT STRIP_TAC THEN
+    Q_TAC SUFF_TAC
+          `!v. ~(v IN ctxtFV G) ==> (v,A)::G ||- [VAR v/x] m -: B`
+          THEN1 METIS_TAC [hastype2_rules] THEN REPEAT STRIP_TAC THEN
+    Cases_on `v = x` THEN1 SRW_TAC [][lemma14a] THEN
+    (* if v = x, proof is trivial; rest of tactic is for other case *)
+    `~(v IN FV m)`
+         by METIS_TAC [hastype2_hastype, hastype_FV, ctxtFV_def,
+                       pairTheory.FST, pred_setTheory.IN_INSERT] THEN
+    `~(x IN ctxtFV G)`
+         by METIS_TAC [hastype2_valid_ctxt, valid_ctxt_def, ctxtFV_MEM] THEN
+    `[VAR v/x] m = swap v x m` by SRW_TAC [][fresh_var_swap] THEN
+    Q_TAC SUFF_TAC
+          `(x,A) :: ctxtswap v x G ||- m -: B`
+          THEN1 SRW_TAC [][hastype2_swap_eqn] THEN
+    SRW_TAC [][ctxtswap_fresh]
+  ]);
+
+val hastype_hastype2_eqn = store_thm(
+  "hastype_hastype2_eqn",
+  ``G |- m -: A = G ||- m -: A``,
+  METIS_TAC [hastype2_hastype, hastype_hastype2]);
 
 val _ = export_theory ()
